Par: Correct formulation of chi + semantic equivalence proof

pulse/examples/steel_wip/Par_Triple.fst
@@ -27,12 +27,41 @@ module Par_Triple
 // Observe that parallel composition `||` is not part of the monad structure, because
 // as is well known (cf the works of Plotkin et al), `||` is in fact a (binary) effect
 // handler defined by recursion on the free monad structure (see below for details).
+
+
+/// Proof sketch for soundness of locks
+///
+/// chi : Hoare triple interpretation of total correctness. Existing implementation, acquire/release encapsulated by get/put
+///
+/// step: state -> c:m a -> Terminates | Block
+///
+/// Total function, does not retry when blocking. If we try to acquire a blocked lock, we directly return blocking.
+/// run_partial : state -> Terminates state | Blocking | Error =
+///   step ...
+///
+/// Partial correctness proof
+/// lemma_chi_characterization
+///   (requires chi c /\ pre c)
+///   (ensures Blocking? (run_partial c h) \/ Terminates? (run_partial /\ post run_partial))
+///
+/// Actual semantics, might not terminate. Blocks while waiting for to acquire locked resource
+/// run: state -> Div (Terminates state | Error)
+///   rec step ...
+///
+/// Final proof: Safety up to n steps of run w.r.t. chi.
+/// This should be achieved using run_partial as an intermediate step
+/// run_partial could be seen as run with "fuel 1", i.e. a non-recursive version
+
+
+
+
+
 noeq
 type m a =
   | Ret : a -> m a
   | Get : bool -> (nat -> m a) -> m a
   | Put : bool -> nat -> m a -> m a
-  | Or  : m a -> m a -> m a
+  | MOr  : m a -> m a -> m a // MOr instead of Or to avoid name clashes with FStar.Reflection
 
 // Functoriality of m
 let rec map (#a:Type) (#b:Type) (f:a -> b) (c:m a) : Tot (m b) (decreases c) =
@@ -40,7 +69,7 @@ let rec map (#a:Type) (#b:Type) (f:a -> b) (c:m a) : Tot (m b) (decreases c) =
   | Ret x -> Ret (f x)
   | Get b c -> Get b (fun n -> FStar.WellFounded.axiom1 c n; map f (c n))
   | Put b n c -> Put b n (map f c)
-  | Or c0 c1 -> Or (map f c0) (map f c1)
+  | MOr c0 c1 -> MOr (map f c0) (map f c1)
 
 
 // Below are two styles of defining the `||` operation. The first of these is more intuitive.
@@ -50,52 +79,33 @@ let rec map (#a:Type) (#b:Type) (f:a -> b) (c:m a) : Tot (m b) (decreases c) =
 val l_par (#a:Type0) (#b:Type0) (c0:m a) (c1:m b) : Tot (m (a & b)) (decreases %[c0;c1])
 val r_par (#a:Type0) (#b:Type0) (c0:m a) (c1:m b) : Tot (m (a & b)) (decreases %[c0;c1])
 
-let rec l_par #a #b c0 c1 =
+let pair_x (#a:Type) (x:a) = fun y -> (x, y)
+let pair_y (#b:Type) (y:b) = fun x -> (x, y)
+
+let rec l_get (#a:Type) (#b:Type) (c0':nat -> m a) (c1:m b) (n:nat) : Tot (m (a & b)) (decreases c0') =
+  FStar.WellFounded.axiom1 c0' n;
+  MOr (l_par (c0' n) c1) (r_par (c0' n) c1)
+
+and l_par #a #b c0 c1 =
   match c0 with
-  | Ret x -> map (fun y -> (x,y)) c1
-  | Get b c0' -> Get b (fun n -> FStar.WellFounded.axiom1 c0' n; Or (l_par (c0' n) c1) (r_par (c0' n) c1))
-  | Put b n c0' -> Put b n (Or (l_par c0' c1) (r_par c0' c1))
-  | Or c0' c0'' -> Or (l_par c0' c1) (l_par c0'' c1)
+  | Ret x -> map (pair_x x) c1
+  | Get b c0' -> Get b (l_get c0' c1)
+  | Put b n c0' -> Put b n (MOr (l_par c0' c1) (r_par c0' c1))
+  | MOr c0' c0'' -> MOr (l_par c0' c1) (l_par c0'' c1)
 
 and r_par #a #b c0 c1 =
   match c1 with
-  | Ret y -> map (fun x -> (x,y)) c0
-  | Get b c1' -> Get b (fun n -> FStar.WellFounded.axiom1 c1' n; Or (l_par c0 (c1' n)) (r_par c0 (c1' n)))
-  | Put b n c1' -> Put b n (Or (l_par c0 c1') (r_par c0 c1'))
-  | Or c1' c1'' -> Or (r_par c0 c1') (r_par c0 c1'')
+  | Ret y -> map (pair_y y) c0
+  | Get b c1' -> Get b (fun n -> FStar.WellFounded.axiom1 c1' n; MOr (l_par c0 (c1' n)) (r_par c0 (c1' n)))
+  | Put b n c1' -> Put b n (MOr (l_par c0 c1') (r_par c0 c1'))
+  | MOr c1' c1'' -> MOr (r_par c0 c1') (r_par c0 c1'')
 
-let m_par (#a #b:Type0) (c0:m a) (c1:m b) =
-  Or (l_par c0 c1) (r_par c0 c1)
+let m_par (#a #b:Type0) (c0:m a) (c1:m b) : m (a & b) =
+  MOr (l_par c0 c1) (r_par c0 c1)
 
-// A logically equivalent definition of parallel composition (at unit)
-// in terms of two unary effect handlers, based on G. Plotkin's slides.
-val r_par' (c0:m unit) (c1:m unit -> m unit) : m unit
-let rec r_par' c0 c1 =
-  match c0 with
-  | Ret x -> Ret x
-  | Get b c0' -> Get b (fun n ->
-                          FStar.WellFounded.axiom1 c0' n;
-                          Or (c1 (c0' n))
-                             (r_par' (c0' n) c1))
-  | Put b n c0' -> Put b n (Or (c1 c0') (r_par' c0' c1))
-  | Or c0' c0'' -> Or (r_par' c0' c1) (r_par' c0'' c1)
+(*** Memory definitions ***)
 
-val l_par' (c0:m unit) (c1:m unit) : m unit
-let rec l_par' c0 c1 =
-  match c0 with
-  | Ret x -> Ret x
-  | Get b c0' -> Get b (fun n ->
-                          FStar.WellFounded.axiom1 c0' n;
-                          Or (l_par' (c0' n) c1)
-                             (r_par' c1 (l_par' (c0' n))))
-  | Put b n c0' -> Put b n (Or (l_par' c0' c1) (r_par' c1 (l_par' c0')))
-  | Or c0' c0'' -> Or (l_par' c0' c1) (l_par' c0'' c1)
-
-let m_par' c0 c1 : m unit =
-  Or (l_par' c0 c1) (r_par' c1 (l_par' c0))
-
-
-// For this example sketch, memory is simply a pair of booleans.
+/// For this example sketch, memory is simply a pair of booleans.
 let mem = bool -> nat
 
 let upd (b:bool) (n:nat) (h:mem) : mem =
@@ -108,30 +118,31 @@ let modifies (fp:loc) (h0 h1:mem) =
   | None -> True
   | Some b -> h0 (not b) == h1 (not b)
 
-// Separating conjunction of two resources.
+/// Separating conjunction of two resources.
 let xor a b = (a || b) && ((not a) || (not b))
 
-// In the current model, two locations are disjoint if they are not the whole memory (None) and if they are actually disjoint (xor of two resources)
+/// In the current model, two locations are disjoint if they are not the whole memory (None) and if they are actually disjoint (xor of two resources)
 let disjoint (l1 l2:loc) = Some? l1 /\ Some? l2 /\ xor (Some?.v l1) (Some?.v l2)
 
-// We only consider predicates that are stable on the resource footprint: They depend only on the memory contents of the available resource
+/// l2 is included in l1
+let includes (l1 l2:loc) =
+  None? l1 \/ // l1 is the whole memory
+  l1 == l2 // Or l1 is Some of something, and l2 needs to be the same
+
+let loc_union (l1 l2:loc) : loc =
+  match l1, l2 with
+  | None, _ | _, None -> None
+  | Some v1, Some v2 -> if v1 = v2 then Some v1 else None
+
+/// We only consider predicates that are stable on the resource footprint: They depend only on the memory contents of the available resource
 let is_stable_on (fp:loc) (pred:mem -> Type) =
-  forall (h0 h1:mem) (l:loc). pred h0 /\ modifies l h0 h1 /\ disjoint fp l ==> pred h1
+  forall (h0 h1:mem) (l:loc). (pred h0 /\ modifies l h0 h1 /\ disjoint fp l) ==> pred h1
 
-// Semantics of the monad
-let rec run #a (c:m a) (h:mem) : a * mem =
-  match c with
-  | Ret x -> x, h
-  | Get b c -> run (FStar.WellFounded.axiom1 c (h b); c (h b)) h
-  | Put b n c -> run c (upd b n h)
-  | Or c0 c1 -> admit()
+(*** Resource definitions ***)
 
-
-// Simple variant of our notion of resources.
+/// Simple variant of our notion of resources.
 let inv_reads_fp (fp:option bool) (inv:mem -> Type0) =
-  match fp with
-  | None -> True
-  | Some b -> forall h h' . inv h /\ modifies (Some (not b)) h h' ==> inv h'
+  forall h h' l. inv h /\ disjoint fp l /\ modifies l h h' ==> inv h'
 
 noeq
 type view_t a = {
@@ -166,41 +177,352 @@ let (<*>) (r0 r1:resource) : resource =
     }
   }
 
+// Cannot leave this function unnamed inside chi definition to reason about it
+let upd_pre (pre:mem -> Type) (b:bool) (n:nat) = fun h -> pre (upd b n h)
 
-// We define the validity of a Hoare triple by induction on a command
-// For the time being, the postcondition only takes one state. TODO: Take initial state as a parameter as well
-// TODO: The postcondition should also take the return value as an argument
-let rec chi #a (c:m a) (r:resource) (pre:mem -> Type) (post:mem -> Type) : Type =
+(*** Axiomatisation of the semantics, RST monad definition ***)
+
+/// We assume here that the initial and final resources are the same
+let rec chi #a (c:m a) (r:resource) (pre:mem -> Type) (post:mem -> Type) (h_init h_current:mem) : Type =
   match c with
-  | Ret x -> forall h. pre h ==> post h
-  | Get b c ->
-    forall h.
-      // TODO: Something about invariant/liveness here?
-      (FStar.WellFounded.axiom1 c (h b);
-      chi (c (h b)) r pre post)
-  | Put b n c -> // TODO: Something about invariant/liveness here?
-        chi c r (fun h -> pre (upd b n h)) post
-  | Or c0 c1 -> chi c0 r pre post /\ chi c1 r pre post
+  | Ret x -> pre h_init ==> post h_current
 
-// This is an alternate characterization of Hoare Triples. This should be provable from the definition of chi.
-// It states that if we satisfy chi, then running the command in a state satisfying the precondition
-// results in a state satisfying the postcondition, and only modifying the specified footprint
-val lemma_chi_characterization (#a:Type) (c:m a) (r:resource) (pre:mem -> Type) (post:mem -> Type) (h0:mem) : Lemma
-  (requires pre h0 /\ chi c r pre post)
+  | Get b c ->
+        includes r.view.fp (Some b) /\ // The accessed memory is inside the resource
+
+        (FStar.WellFounded.axiom1 c (h_current b);
+        chi (c (h_current b)) r pre post h_init h_current)
+
+  | Put b n c ->
+        includes r.view.fp (Some b) /\ // The updated memory is inside the resource
+        // TODO: Equivalence is probably too strong. Should we rephrase chi to be {r.view.inv /\ pre}c{post /\ r.view.inv}
+        // with resource invariants somehow outside of chi?
+        (r.view.inv h_current <==> r.view.inv (upd b n h_current)) /\ // The resource invariant is preserved
+
+        chi c r pre post h_init (upd b n h_current)
+
+  | MOr c0 c1 -> chi c0 r pre post h_init h_current /\ chi c1 r pre post h_init h_current
+
+
+let r_pred (pred:mem -> Type) (r:resource) = fun h -> pred h /\ r.view.inv h
+
+/// The `is_stable_on predicate` is not yet provable in the current RST model:
+/// pre/postconditions can currently refer to the whole memory, and not just the resource footprint
+/// This will be resolved once selectors are implemented
+let rst (a:Type) (r:resource) (pre post:mem -> Type) = c:m a{
+  (forall h. chi c r (r_pred pre r) (r_pred post r) h h) /\
+  is_stable_on r.view.fp pre /\ is_stable_on r.view.fp post}
+
+(*** Denotational semantics ***)
+
+
+/// Semantics of the monad
+/// To resolve non-determinism for MOr, we might need a stream of booleans to pick the left or right branch at each or instruction
+let rec run #a (c:m a) (h:mem) (pos:nat) (stream:nat -> bool) : a * mem =
+  match c with
+  | Ret x -> x, h
+  | Get b c -> run (FStar.WellFounded.axiom1 c (h b); c (h b)) h pos stream
+  | Put b n c -> run c (upd b n h) pos stream
+  | MOr c0 c1 -> match stream pos with
+                | false -> run c0 h (pos + 1) stream
+                | true -> run c1 h (pos + 1) stream
+
+/// The denotational semantics `run` and their axiomatisation `chi` should be coherent
+/// More precisely, if we satisfy chi, then running the command `c` in a state satisfying the precondition
+/// results in a state satisfying the postcondition, and only modifying the specified footprint
+/// This would prove that Hoare triples accepted by chi always match the semantics
+val lemma_chi_characterization (#a:Type) (c:m a) (r:resource) (pre:mem -> Type) (post:mem -> Type) (h0:mem) (pos:nat) (stream:nat -> bool) : Lemma
+  (requires pre h0 /\ chi c r pre post h0 h0)
   (ensures (
-    let x, h1 = run c h0 in
+    let x, h1 = run c h0 pos stream in
     post h1 /\ modifies r.view.fp h0 h1)
   )
 
-let lemma_chi_characterization #a c pre post h0 = admit()
+val lemma_chi_characterization_aux (#a:Type) (c:m a) (r:resource) (pre:mem -> Type) (post:mem -> Type) (h0 h_current:mem) (pos:nat) (stream:nat -> bool) : Lemma
+  (requires pre h0 /\ chi c r pre post h0 h_current)
+  (ensures (
+    let x, h1 = run c h_current pos stream in
+    post h1 /\ modifies r.view.fp h_current h1)
+  )
 
-let rst (a:Type) (r:resource) (pre post:mem -> Type) = c:m a{chi c r pre post}
 
-val par  (#a #b:Type)
-         (#r0 #r1:resource)
+let rec lemma_chi_characterization_aux #a c r pre post h0 h_current pos stream =
+  match c with
+  | Ret x -> ()
+  | Get b c -> FStar.WellFounded.axiom1 c (h_current b); lemma_chi_characterization_aux (c (h_current b)) r pre post h0 h_current pos stream
+  | Put b n c -> lemma_chi_characterization_aux c r pre post h0 (upd b n h_current) pos stream
+  | MOr c0 c1 -> match stream pos with
+    | false -> lemma_chi_characterization_aux c0 r pre post h0 h_current (pos + 1) stream
+    | true -> lemma_chi_characterization_aux c1 r pre post h0 h_current (pos + 1) stream
+
+let lemma_chi_characterization #a c r pre post h0 pos stream = lemma_chi_characterization_aux #a c r pre post h0 h0 pos stream
+
+(*** Lemmas about chi ***)
+
+(* TODO: Restore this
+
+/// Map preserves chi
+let rec map_chi (#a:Type) (#b:Type) (f:a -> b) (c:m a) (r:resource) (pre:mem -> Type) (post:mem -> Type) :
+  Lemma
+  (requires chi c r pre post)
+  (ensures chi (map f c) r pre post)
+  (decreases c) =
+  match c with
+  | Ret x -> ()
+  | Get b c' ->
+        let aux (h:mem) : Lemma (chi (map f (c' (h b))) r pre post)
+          = FStar.WellFounded.axiom1 c' (h b); map_chi f (c' (h b)) r pre post
+        in Classical.forall_intro aux
+  | Put b n c -> map_chi f c r (upd_pre pre b n) post
+  | MOr c0 c1 -> map_chi f c0 r pre post; map_chi f c1 r pre post
+
+/// We can derive a weaker precondition from a stronger one
+let rec chi_weaken_post (#a:Type) (c:m a) (r:resource) (pre:mem -> Type) (post:mem -> Type) (post_weak:mem -> Type)
+  : Lemma
+  (requires chi c r pre post /\ (forall h. post h ==> post_weak h))
+  (ensures chi c r pre post_weak)
+  (decreases c) =
+  match c with
+  | Ret _ -> ()
+  | Get b c' ->
+    let aux (h:mem) : Lemma (chi (c' (h b)) r pre post_weak)
+      = FStar.WellFounded.axiom1 c' (h b); chi_weaken_post (c' (h b)) r pre post post_weak
+    in Classical.forall_intro aux
+  | Put b n c -> chi_weaken_post c r (upd_pre pre b n) post post_weak
+  | MOr c0 c1 -> chi_weaken_post c0 r pre post post_weak; chi_weaken_post c1 r pre post post_weak
+
+/// chi still holds if we strengthen the precondition
+let rec chi_stronger_pre (#a:Type) (c:m a) (r:resource) (pre:mem -> Type) (post:mem -> Type) (pre_strong:mem -> Type)
+  : Lemma
+  (requires chi c r pre post /\ (forall h. pre_strong h ==> pre h))
+  (ensures chi c r pre_strong post)
+  (decreases c) =
+  match c with
+  | Ret _ -> ()
+  | Get b c' ->
+    let aux (h:mem) : Lemma (chi (c' (h b)) r pre_strong post)
+      = FStar.WellFounded.axiom1 c' (h b); chi_stronger_pre (c' (h b)) r pre post pre_strong
+    in Classical.forall_intro aux
+  | Put b n c -> chi_stronger_pre c r (upd_pre pre b n) post (upd_pre pre_strong b n)
+  | MOr c0 c1 -> chi_stronger_pre c0 r pre post pre_strong; chi_stronger_pre c1 r pre post pre_strong
+
+/// If a subset of pre implies a new post for any memory, then chi still holds when the new post is added to the existing postcondition
+let rec chi_pre_implies_post (#a:Type) (c:m a) (r:resource) (l:loc) (pre:mem -> Type) (pre_small:mem -> Type) (post:mem -> Type) (post_add:mem -> Type)
+  : Lemma
+  (requires chi c r pre post /\
+            (forall h. pre h ==> pre_small h) /\
+            (forall h. pre_small h ==> post_add h) /\
+            is_stable_on l pre_small /\
+            is_stable_on l post_add /\
+            disjoint l r.view.fp)
+  (ensures chi c r pre (fun h -> post h /\ post_add h))
+  (decreases c) =
+  match c with
+  | Ret _ -> ()
+  | Get b c' ->
+    let aux (h:mem) : Lemma (chi (c' (h b)) r pre (fun h -> post h /\ post_add h))
+      = FStar.WellFounded.axiom1 c' (h b); chi_pre_implies_post (c' (h b)) r l pre pre_small post post_add
+    in Classical.forall_intro aux
+  | Put b n c ->
+    let aux (h:mem) : Lemma
+      (requires upd_pre pre_small b n h)
+      (ensures pre_small h)
+      = let h' = upd b n h in
+        assert (modifies r.view.fp h' h)
+    in Classical.forall_intro (Classical.move_requires aux);
+    let aux_stable (h0 h1:mem) (l':loc) : Lemma
+      (requires upd_pre pre_small b n h0 /\ modifies l' h0 h1 /\ disjoint l' l)
+      (ensures upd_pre pre_small b n h1)
+      = let h0' = upd b n h0 in
+        let h1' = upd b n h1 in
+        assert (modifies (loc_union r.view.fp l') h0' h1')
+    in Classical.forall_intro_3 (fun h0 h1 l -> Classical.move_requires (aux_stable h0 h1) l);
+    chi_pre_implies_post c r l (upd_pre pre b n) (upd_pre pre_small b n) post post_add
+  | MOr c0 c1 -> chi_pre_implies_post c0 r l pre pre_small post post_add; chi_pre_implies_post c1 r l pre pre_small post post_add
+
+/// We can extend the resource in chi to a starred resource
+let rec chi_bigger_resource (#a:Type) (c:m a) (r0 r1:resource) (pre:mem -> Type) (post:mem -> Type)
+  : Lemma
+  (requires chi c r1 pre post /\ disjoint r0.view.fp r1.view.fp)
+  (ensures chi c (r0 <*> r1) pre post /\ chi c (r1 <*> r0) pre post)
+  (decreases c)
+  =  match c with
+  | Ret _ -> ()
+  | Get b c' ->
+    let aux (h:mem) : Lemma (chi (c' (h b)) (r0 <*> r1) pre post /\ chi (c' (h b)) (r1 <*> r0) pre post)
+      = FStar.WellFounded.axiom1 c' (h b); chi_bigger_resource (c' (h b)) r0 r1 pre post
+    in Classical.forall_intro aux
+  | Put b n c ->
+      let aux (h:mem) : Lemma
+      (ensures r0.view.inv h <==> r0.view.inv (upd b n h))
+      =
+      let h' = upd b n h in
+      assert (modifies (r1.view.fp) h h');
+      assert (modifies r1.view.fp h' h)
+    in Classical.forall_intro (Classical.move_requires aux);
+    chi_bigger_resource c r0 r1 (upd_pre pre b n) post
+  | MOr c0 c1 -> chi_bigger_resource c0 r0 r1 pre post; chi_bigger_resource c1 r0 r1 pre post
+
+let rec lemma_lpar (#a #b:Type)
+    (r0:resource) (r1:resource{disjoint r0.view.fp r1.view.fp})
+    (c0:m a) (c1:m b)
+    (pre0 pre1 post0 post1:mem -> Type) : Lemma
+    (requires chi c0 r0 (r_pred pre0 r0) (r_pred post0 r0) /\ is_stable_on r0.view.fp pre0 /\ is_stable_on r0.view.fp post0 /\
+      chi c1 r1 (r_pred pre1 r1) (r_pred post1 r1) /\ is_stable_on r1.view.fp pre1 /\ is_stable_on r1.view.fp post1)
+    (ensures chi (l_par c0 c1) (r0 <*> r1) (r_pred (fun h -> pre0 h /\ pre1 h) (r0 <*> r1)) (r_pred (fun h -> post0 h /\ post1 h) (r0 <*> r1)))
+    (decreases %[c0; c1])
+    = match c0 with
+    | Ret x ->
+      map_chi (pair_x x) c1 r1 (r_pred pre1 r1) (r_pred post1 r1);
+      chi_stronger_pre (l_par c0 c1) r1 (r_pred pre1 r1) (r_pred post1 r1) (r_pred (fun h -> pre0 h /\ pre1 h) (r0 <*> r1));
+      chi_pre_implies_post (l_par c0 c1) r1 r0.view.fp
+        (r_pred (fun h -> pre0 h /\ pre1 h) (r0 <*> r1))
+        (r_pred pre0 r0)
+        (r_pred post1 r1) (r_pred post0 r0);
+      chi_weaken_post (l_par c0 c1) r1 (r_pred (fun h -> pre0 h /\ pre1 h) (r0 <*> r1))
+        (fun h -> r_pred post1 r1 h /\ r_pred post0 r0 h) (r_pred (fun h -> post0 h /\ post1 h) (r0 <*> r1));
+      chi_bigger_resource (l_par c0 c1) r0 r1 (r_pred (fun h -> pre0 h /\ pre1 h) (r0 <*> r1)) (r_pred (fun h -> post0 h /\ post1 h) (r0 <*> r1))
+
+    | Get b' c0' ->
+      let aux (h:mem) : Lemma (chi (MOr (l_par (c0' (h b')) c1) (r_par (c0' (h b')) c1)) (r0 <*> r1)
+        (r_pred (fun h -> pre0 h /\ pre1 h) (r0 <*> r1)) (r_pred (fun h -> post0 h /\ post1 h) (r0 <*> r1)))
+      = FStar.WellFounded.axiom1 c0' (h b');
+        lemma_lpar r0 r1 (c0' (h b')) c1 pre0 pre1 post0 post1;
+        lemma_rpar r0 r1 (c0' (h b')) c1 pre0 pre1 post0 post1
+      in
+      Classical.forall_intro aux
+
+    | Put b' n c0' ->
+      let r = r0 <*> r1 in
+      chi_stronger_pre c0' r0 (upd_pre (r_pred pre0 r0) b' n) (r_pred post0 r0) (r_pred (upd_pre pre0 b' n) r0);
+
+      let aux_stable (h0 h1:mem) (l':loc) : Lemma
+        (requires upd_pre pre0 b' n h0 /\ modifies l' h0 h1 /\ disjoint l' r0.view.fp)
+        (ensures upd_pre pre0 b' n h1)
+        = let h0' = upd b' n h0 in
+          let h1' = upd b' n h1 in
+          assert (modifies l' h0' h1')
+
+      in Classical.forall_intro_3 (fun h0 h1 l -> Classical.move_requires (aux_stable h0 h1) l);
+
+      lemma_lpar r0 r1 c0' c1 (upd_pre pre0 b' n) pre1 post0 post1;
+      lemma_rpar r0 r1 c0' c1 (upd_pre pre0 b' n) pre1 post0 post1;
+
+
+      let aux (h:mem) : Lemma
+        (requires upd_pre (r_pred (fun h -> pre0 h /\ pre1 h) (r0 <*> r1)) b' n h)
+        (ensures r_pred (fun h -> upd_pre pre0 b' n h /\ pre1 h) (r0 <*> r1) h)
+        = let h' = upd b' n h in
+          assert (modifies r0.view.fp h (upd b' n h));
+          assert (modifies r0.view.fp h' h)
+      in
+      Classical.forall_intro (Classical.move_requires aux);
+      chi_stronger_pre (l_par c0' c1) (r0 <*> r1)
+        (r_pred (fun h -> (upd_pre pre0 b' n) h /\ pre1 h) (r0 <*> r1))
+        (r_pred (fun h -> post0 h /\ post1 h) (r0 <*> r1))
+        (upd_pre (r_pred (fun h -> pre0 h /\ pre1 h) (r0 <*> r1)) b' n);
+      chi_stronger_pre (r_par c0' c1) (r0 <*> r1)
+        (r_pred (fun h -> (upd_pre pre0 b' n) h /\ pre1 h) (r0 <*> r1))
+        (r_pred (fun h -> post0 h /\ post1 h) (r0 <*> r1))
+        (upd_pre (r_pred (fun h -> pre0 h /\ pre1 h) (r0 <*> r1)) b' n);
+
+      let aux (h:mem) : Lemma
+        (ensures r.view.inv h <==> r.view.inv (upd b' n h))
+        = assert (modifies r0.view.fp h (upd b' n h)); assert (modifies r0.view.fp (upd b' n h) h)
+      in
+      Classical.forall_intro (Classical.move_requires aux)
+
+
+    | MOr c0' c0'' -> lemma_lpar r0 r1 c0' c1 pre0 pre1 post0 post1; lemma_lpar r0 r1 c0'' c1 pre0 pre1 post0 post1
+
+and lemma_rpar (#a #b:Type)
+    (r0:resource) (r1:resource{disjoint r0.view.fp r1.view.fp})
+    (c0:m a) (c1:m b)
+    (pre0 pre1 post0 post1:mem -> Type) : Lemma
+    (requires chi c0 r0 (r_pred pre0 r0) (r_pred post0 r0) /\ is_stable_on r0.view.fp pre0 /\ is_stable_on r0.view.fp post0 /\
+      chi c1 r1 (r_pred pre1 r1) (r_pred post1 r1) /\ is_stable_on r1.view.fp pre1 /\ is_stable_on r1.view.fp post1)
+    (ensures chi (r_par c0 c1) (r0 <*> r1) (r_pred (fun h -> pre0 h /\ pre1 h) (r0 <*> r1)) (r_pred (fun h -> post0 h /\ post1 h) (r0 <*> r1)))
+    (decreases %[c0; c1])
+    = match c1 with
+    | Ret y ->
+      map_chi (pair_y y) c0 r0 (r_pred pre0 r0) (r_pred post0 r0);
+      chi_stronger_pre (r_par c0 c1) r0 (r_pred pre0 r0) (r_pred post0 r0) (r_pred (fun h -> pre0 h /\ pre1 h) (r0 <*> r1));
+      chi_pre_implies_post (r_par c0 c1) r0 r1.view.fp
+        (r_pred (fun h -> pre0 h /\ pre1 h) (r0 <*> r1))
+        (r_pred pre1 r1)
+        (r_pred post0 r0) (r_pred post1 r1);
+      chi_weaken_post (r_par c0 c1) r0 (r_pred (fun h -> pre0 h /\ pre1 h) (r0 <*> r1))
+        (fun h -> r_pred post0 r0 h /\ r_pred post1 r1 h) (r_pred (fun h -> post0 h /\ post1 h) (r0 <*> r1));
+      chi_bigger_resource (r_par c0 c1) r1 r0 (r_pred (fun h -> pre0 h /\ pre1 h) (r0 <*> r1)) (r_pred (fun h -> post0 h /\ post1 h) (r0 <*> r1))
+
+    | Get b' c1' ->
+      let aux (h:mem) : Lemma (chi (MOr (l_par c0 (c1' (h b'))) (r_par c0 (c1' (h b')))) (r0 <*> r1)
+        (r_pred (fun h -> pre0 h /\ pre1 h) (r0 <*> r1)) (r_pred (fun h -> post0 h /\ post1 h) (r0 <*> r1)))
+      = FStar.WellFounded.axiom1 c1' (h b');
+        lemma_lpar r0 r1 c0 (c1' (h b')) pre0 pre1 post0 post1;
+        lemma_rpar r0 r1 c0 (c1' (h b')) pre0 pre1 post0 post1
+      in
+      Classical.forall_intro aux
+
+    | Put b' n c1' ->
+      let r = r0 <*> r1 in
+      chi_stronger_pre c1' r1 (upd_pre (r_pred pre1 r1) b' n) (r_pred post1 r1) (r_pred (upd_pre pre1 b' n) r1);
+
+      let aux_stable (h0 h1:mem) (l':loc) : Lemma
+          (requires upd_pre pre1 b' n h0 /\ modifies l' h0 h1 /\ disjoint l' r1.view.fp)
+          (ensures upd_pre pre1 b' n h1)
+          = let h0' = upd b' n h0 in
+            let h1' = upd b' n h1 in
+            assert (modifies l' h0' h1')
+
+      in Classical.forall_intro_3 (fun h0 h1 l -> Classical.move_requires (aux_stable h0 h1) l);
+
+      lemma_lpar r0 r1 c0 c1' pre0 (upd_pre pre1 b' n) post0 post1;
+      lemma_rpar r0 r1 c0 c1' pre0 (upd_pre pre1 b' n) post0 post1;
+
+      let aux (h:mem) : Lemma
+        (requires upd_pre (r_pred (fun h -> pre0 h /\ pre1 h) (r0 <*> r1)) b' n h)
+        (ensures r_pred (fun h -> pre0 h /\ upd_pre pre1 b' n h) (r0 <*> r1) h)
+        = let h' = upd b' n h in
+          assert (modifies r1.view.fp h (upd b' n h));
+          assert (modifies r1.view.fp h' h)
+      in
+      Classical.forall_intro (Classical.move_requires aux);
+
+      chi_stronger_pre (l_par c0 c1') (r0 <*> r1)
+        (r_pred (fun h -> pre0 h /\ (upd_pre pre1 b' n) h) (r0 <*> r1))
+        (r_pred (fun h -> post0 h /\ post1 h) (r0 <*> r1))
+        (upd_pre (r_pred (fun h -> pre0 h /\ pre1 h) (r0 <*> r1)) b' n);
+      chi_stronger_pre (r_par c0 c1') (r0 <*> r1)
+        (r_pred (fun h -> pre0 h /\ (upd_pre pre1 b' n) h) (r0 <*> r1))
+        (r_pred (fun h -> post0 h /\ post1 h) (r0 <*> r1))
+        (upd_pre (r_pred (fun h -> pre0 h /\ pre1 h) (r0 <*> r1)) b' n);
+
+      let aux (h:mem) : Lemma
+        (ensures r.view.inv h <==> r.view.inv (upd b' n h))
+        = assert (modifies r1.view.fp h (upd b' n h)); assert (modifies r1.view.fp (upd b' n h) h)
+      in
+    Classical.forall_intro (Classical.move_requires aux)
+
+    | MOr c1' c1'' -> lemma_rpar r0 r1 c0 c1' pre0 pre1 post0 post1; lemma_rpar r0 r1 c0 c1'' pre0 pre1 post0 post1
+
+(*** Parallel composition ***)
+
+/// This is where we enforce that we can only perform parallel composition of commands operating on resources with disjoint footprints
+/// If memory footprints overlapped, we wouldn't be able to prove that assuming only both preconditions, we can prove both postconditions
+/// through any interleaving (modeled by chi)
+val par  (#a #b:Type0)
+         (#r0:resource)
+         (#r1:resource{disjoint r0.view.fp r1.view.fp})
          (#pre0 #pre1 #post0 #post1:mem -> Type)
          (c0:rst a r0 pre0 post0)
          (c1:rst b r1 pre1 post1)
        : rst (a & b) (r0 <*> r1) (fun h -> pre0 h /\ pre1 h) (fun h -> post0 h /\ post1 h)
 
-let par #a #b #r0 #r1 #pre0 #pre1 #post0 #post1 c0 c1 = admit()
+let par #a #b #r0 #r1 #pre0 #pre1 #post0 #post1 c0 c1 =
+  let c = m_par c0 c1 in
+  (**) lemma_lpar r0 r1 c0 c1 pre0 pre1 post0 post1;
+  (**) lemma_rpar r0 r1 c0 c1 pre0 pre1 post0 post1;
+  c
+
+*)
